iris/UkCatMain.v
@@ -785,7 +785,7 @@ Section UkCatMain.
         rewrite Hh32. lia. }
       iApply (wp_kcat_close N Hpsok_free h10 m9 fd (FdOpen rd wr t)
                 (8 + (10 + (12 + (4 + n)))) Ha0_9
-                with "Hcode Hrun Hh").
+                with "Hdp Hcode Hrun Hh").
       iIntros (h11 ret2) "Hrun".
       assert (Eclose : ret_pc (m9 !!! Regidx ra_idx)
                        = (mword_of_int 0xc0 : mword 64))
